made conditional_add a wrapper, defined and proved sub_then_maybe_add

src/Arithmetic/Saturated.v
@@ -515,59 +515,17 @@ Module Columns.
         (fun PQ => from_associational_cps weight n3 PQ
         (fun R => compact_cps (div:=div) (modulo:=modulo) (add_get_carry:=Z.add_get_carry_full) weight R f)))).
 
-  End Wrappers.
-  Hint Unfold add_cps unbalanced_sub_cps mul_cps.
-
-  (* These come after the wrapper definitions because they depend on
-     e.g. unbalanced_sub and add. *)
-  Section Conditionals.
-    Context (weight : nat->Z)
-            {weight_0 : weight 0%nat = 1}
-            {weight_nonzero : forall i, weight i <> 0}
-            {weight_positive : forall i, weight i > 0}
-            {weight_multiples : forall i, weight (S i) mod weight i = 0}
-            {weight_divides : forall i : nat, weight (S i) / weight i > 0}
-    .
-    
-    Definition conditional_add_cps {n} mask cond (p q : Z^n)
+    Definition conditional_add_cps {n1 n2 n3} mask cond (p:Z^n1) (q:Z^n2)
                {T} (f:_->T) :=
       B.Positional.select_cps mask cond q
-                 (fun qq => add_cps (n3:=n) weight p qq f).
-    Definition conditional_add {n} mask cond p q :=
-      @conditional_add_cps n mask cond p q _ id.
-    Lemma conditional_add_id {n} mask cond p q T f:
-      @conditional_add_cps n mask cond p q T f
-      = f (conditional_add mask cond p q).
-    Proof.
-      cbv [conditional_add_cps conditional_add]; autounfold;
-        autorewrite with push_id uncps; reflexivity.
-    Qed.
-    Hint Opaque conditional_add : uncps.
-    Hint Rewrite @conditional_add_id : uncps.
+                 (fun qq => add_cps (n3:=n3) p qq f).
 
-    Lemma eval_conditional_add {n} mask cond p q (n_nonzero:n<>0%nat)
-      (H:Tuple.map (Z.land mask) q = q) :
-    B.Positional.eval weight (snd (@conditional_add n mask cond p q))
-    = B.Positional.eval weight p + (if (dec (cond = 0)) then 0 else B.Positional.eval weight q) - weight n * (fst (conditional_add mask cond p q)).
-  Proof.
-    cbv [conditional_add_cps conditional_add];
-      repeat progress autounfold in *. cbv [add_cps].
-    pose proof Z.add_get_carry_full_mod.
-    pose proof Z.add_get_carry_full_div.
-    pose proof div_correct. pose proof modulo_correct.
-    autorewrite with uncps push_id push_basesystem_eval.
-    break_match;
-      match goal with
-        |- context [weight ?n * (?x / weight ?n)] =>
-        pose proof (Z.div_mod x (weight n) (weight_nonzero n))
-      end; omega.
-  Qed.
-  Hint Rewrite @eval_conditional_add using (omega || assumption)
-    : push_basesystem_eval.
-  End Conditionals.
-  
+  End Wrappers.
+  Hint Unfold add_cps unbalanced_sub_cps mul_cps conditional_add_cps.
+
 End Columns.
 Hint Unfold
+     Columns.conditional_add_cps
      Columns.add_cps
      Columns.unbalanced_sub_cps
      Columns.mul_cps.
@@ -577,7 +535,6 @@ Hint Rewrite
      @Columns.compact_id
      @Columns.cons_to_nth_id
      @Columns.from_associational_id
-     @Columns.conditional_add_id
   : uncps.
 Hint Rewrite
      @Columns.compact_mod
@@ -585,7 +542,6 @@ Hint Rewrite
      @Columns.eval_cons_to_nth
      @Columns.eval_from_associational
      @Columns.eval_nils
-     @Columns.eval_conditional_add
   using (assumption || omega): push_basesystem_eval.
 
 Section Freeze.
@@ -614,8 +570,8 @@ Section Freeze.
     the carry in step 3 was -1, so they cancel out.
    *)
   Definition freeze_cps {n} mask (m:Z^n) (p:Z^n) {T} (f : Z^n->T) :=
-    Columns.unbalanced_sub_cps weight p m
-      (fun carry_p => Columns.conditional_add_cps weight mask (fst carry_p) (snd carry_p) m
+    Columns.unbalanced_sub_cps (n3:=n) weight p m
+      (fun carry_p => Columns.conditional_add_cps (n3:=n) weight mask (fst carry_p) (snd carry_p) m
       (fun carry_r => f (snd carry_r)))
   .
 
@@ -669,7 +625,7 @@ Section Freeze.
              (B.Positional.eval weight (@freeze n mask m p))
              (B.Positional.eval weight p).
   Proof.
-    cbv [freeze_cps freeze Columns.conditional_add_cps].
+    cbv [freeze_cps freeze].
     repeat progress autounfold.
     pose proof Z.add_get_carry_full_mod.
     pose proof Z.add_get_carry_full_div.
@@ -751,9 +707,21 @@ Section API.
       f).
   Definition add {n m pred_nm} p q : T (S pred_nm) := @add_cps n m pred_nm p q _ id.
 
+  Definition sub_then_maybe_add_cps {n} mask (p q r : T n) {R} (f:T n -> R) :=
+    Columns.unbalanced_sub_cps (n3:=n) (uweight bound) p q
+      (* the carry will be 0 unless we underflow--we do the addition only
+         in the underflow case *)
+      (fun carry_result =>
+         Columns.conditional_add_cps (uweight bound) mask (fst carry_result) (left_append (fst carry_result) (snd carry_result)) r
+      (* We can now safely discard the carry. This relies on the
+         precondition that p - q + r < bound^n. *)
+      (fun carry_result' => f (snd carry_result'))).
+  Definition sub_then_maybe_add {n} mask (p q r : T n) :=
+    sub_then_maybe_add_cps mask p q r id.
+
    (* Subtract q if and only if p < bound^n. The correctness of this
   lemma depends on the precondition that p < q + bound^n.  *)
-  Definition conditional_sub_cps {n} (p : Z^S n) (q : Z ^ n)
+  Definition conditional_sub_cps {n} mask (p : Z^S n) (q : Z ^ n)
              {T} (f:Z^n->T) :=
       (* we pass the highest digit of p into select_cps as the
       conditional argument; if it is 0, the subtraction will not
@@ -768,7 +736,7 @@ Section API.
 
   Definition conditional_sub {n} mask p q := @conditional_sub_cps n mask p q _ id.
 
-  Hint Opaque join0 divmod drop_high scmul add conditional_sub : uncps.
+  Hint Opaque join0 divmod drop_high scmul add sub_then_maybe_add conditional_sub : uncps.
 
   Section CPSProofs.
 
@@ -796,12 +764,16 @@ Section API.
       @add_cps n m pred_nm p q R f = f (add p q).
     Proof. cbv [add_cps add Let_In]. prove_id. Qed.
 
+    Lemma sub_then_maybe_add_id n mask p q r R f :
+      @sub_then_maybe_add_cps n mask p q r R f = f (sub_then_maybe_add mask p q r).
+    Proof. cbv [sub_then_maybe_add_cps sub_then_maybe_add Let_In]. prove_id. Qed.
+
     Lemma conditional_sub_id n mask p q R f :
       @conditional_sub_cps n mask p q R f = f (conditional_sub mask p q).
     Proof. cbv [conditional_sub_cps conditional_sub Let_In]. prove_id. Qed.
 
   End CPSProofs.
-  Hint Rewrite join0_id divmod_id drop_high_id scmul_id add_id conditional_sub_id : uncps.
+  Hint Rewrite join0_id divmod_id drop_high_id scmul_id add_id sub_then_maybe_add_id conditional_sub_id : uncps.
 
   Section Proofs.
 
@@ -1038,6 +1010,67 @@ Section API.
       apply small_left_tl.
     Qed.
 
+    Lemma div_nonzero_neg_iff x y : x < y -> 0 < y -> x / y <> 0 <-> x < 0.
+    Proof.
+      repeat match goal with
+             | _ => progress intros
+             | _ => rewrite Z.div_small_iff by omega
+             | _ => split
+             | _ => omega
+             end.
+   Qed.
+
+    Lemma eval_sub_then_maybe_add_nz n mask p q r:
+      small p -> small q -> small r -> (n<>0)%nat ->
+      (map (Z.land mask) r = r) ->
+      (0 <= eval p < eval r) -> (0 <= eval q < eval r) ->
+      eval (@sub_then_maybe_add n mask p q r) = eval p - eval q + (if eval p - eval q <? 0 then eval r else 0).
+    Proof.
+      pose_all.
+      repeat match goal with
+             | _ => progress (cbv [sub_then_maybe_add sub_then_maybe_add_cps eval] in *; intros)
+             | _ => progress autounfold
+             | _ => progress autorewrite with uncps push_id push_basesystem_eval
+             | H : small _ |- _ => apply eval_small in H
+             | _ => progress break_match
+             | _ => (rewrite Z.add_opp_r in * )
+             | _ => progress autorewrite with zsimplify; [ ]
+             | H : _ |- _ => rewrite Z.ltb_lt in H;
+                               rewrite <-div_nonzero_neg_iff with
+                               (y:=uweight bound n) in H by (auto; omega)
+             | H : _ |- _ => rewrite Z.ltb_ge in H
+             | _ => rewrite Z.mod_small by omega
+             | _ => omega
+             end;
+      repeat match goal with
+             | H : _ |- _ => rewrite div_nonzero_neg_iff in H
+                 by (auto; omega)
+             | |- context [-?x + ?y mod ?x] =>
+               replace (-x + y mod x) with y
+                 by (rewrite Z.mod_eq, Z.div_small_neg; omega)
+             | _ => apply Z.mod_small; omega
+             | _ => omega
+             end.
+    Qed.
+    
+    Lemma eval_sub_then_maybe_add n mask p q r:
+      small p -> small q -> small r ->
+      (map (Z.land mask) r = r) ->
+      (0 <= eval p < eval r) -> (0 <= eval q < eval r) ->
+      eval (@sub_then_maybe_add n mask p q r) = eval p - eval q + (if eval p - eval q <? 0 then eval r else 0).
+    Proof.
+      destruct n; [|solve[auto using eval_sub_then_maybe_add_nz]].
+      destruct p, q, r; reflexivity.
+    Qed.
+    
+   Lemma small_sub_then_maybe_add n mask (p q r : T n) :
+      small (sub_then_maybe_add mask p q r).
+   Proof.
+     cbv [sub_then_maybe_add_cps sub_then_maybe_add]; intros.
+     repeat progress autounfold. autorewrite with uncps push_id.
+     apply small_compact.
+   Qed. 
+
     Lemma small_highest_zero_iff {n} (p: T (S n)) (Hsmall : small p) :
       (left_hd p = 0 <-> eval p < uweight bound n).
     Proof.
@@ -1148,7 +1181,7 @@ Section API.
 
   End Proofs.
 End API.
-Hint Rewrite join0_id divmod_id drop_high_id scmul_id add_id conditional_sub_id : uncps.
+Hint Rewrite join0_id divmod_id drop_high_id scmul_id add_id sub_then_maybe_add_id conditional_sub_id : uncps.
 
 (*
 (* Just some pretty-printing *)
